\section{Local maxima, local minima, and derivatives}\label{sec 10.2}

\begin{definition}[Local maxima and minima]\label{10.2.1}
    Let \(X\) be a subset of \(\mathbf{R}\), and let \(f : X \to \mathbf{R}\) be a function, and let \(x_0 \in X\).
    We say that \(f\) attains a \emph{local maximum} at \(x_0\) iff there exists a \(\delta > 0\) such that the restriction \(f|_{X \cap (x_0 - \delta, x_0 + \delta)}\) of \(f\) to \(X \cap (x_0 - \delta, x_0 + \delta)\) attains a maximum at \(x_0\).
    We say that \(f\) attains a \emph{local minimum} at \(x_0\) iff there exists a \(\delta > 0\) such that the restriction \(f|_{X \cap (x_0 - \delta, x_0 + \delta)}\) of \(f\) to \(X \cap (x_0 - \delta, x_0 + \delta)\) attains a minimum at \(x_0\).
\end{definition}

\begin{remark}\label{10.2.2}
    If \(f\) attains a maximum at \(x_0\), we sometimes say that \(f\) attains a \emph{global} maximum at \(x_0\), in order to distinguish it from the local maxima defined in Definition \ref{10.2.1}.
    Note that if \(f\) attains a global maximum at \(x_0\), then it certainly also attains a local maximum at this \(x_0\), and similarly for minima.
\end{remark}

\setcounter{theorem}{4}
\begin{remark}\label{10.2.5}
    If \(f : X \to \mathbf{R}\) attains a local maximum at a point \(x_0\) in \(X\), and \(Y \subseteq X\) is a subset of \(X\) which contains \(x_0\), then the restriction \(f|_Y : Y \to \mathbf{R}\) also attains a local maximum at \(x_0\).
    Similarly for minima.
\end{remark}

\begin{proposition}[Local extrema are stationary]\label{10.2.6}
    Let \(a < b\) be real numbers, and let \(f : (a, b) \to \mathbf{R}\) be a function.
    If \(x_0 \in (a, b)\), \(f\) is differentiable at \(x_0\), and \(f\) attains either a local maximum or local minimum at \(x_0\), then \(f'(x_0) = 0\).
\end{proposition}

\begin{proof}
    Suppose \(f\) attains local maximum at \(x_0\).
    Then by Definition \ref{10.2.1} we know that
    \[
        \exists\ \delta \in \mathbf{R}^+ : \forall\ x \in (a, b) \cap (x_0 - \delta, x_0 + \delta), f(x) \leq f(x_0).
    \]
    Since \(f\) is differentiable at \(x_0\), by Definition \ref{10.1.1} we know that
    \[
        \lim_{x \to x_0 ; x \in (a, b) \setminus \{x_0\}} \frac{f(x) - f(x_0)}{x - x_0} = f'(x_0)
    \]
    By Definition \ref{9.3.6} we know that \(\forall\ \varepsilon \in \mathbf{R}^+\), \(\exists\ \delta' \in \mathbf{R}^+\) such that
    \[
        \forall\ x \in (a, b) \setminus \{x_0\}, \abs*{x - x_0} < \delta' \implies \abs*{\frac{f(x) - f(x_0)}{x - x_0} - f'(x_0)} \leq \varepsilon.
    \]
    In particular, we have
    \[
        \forall\ x \in (a, b) \cap (x_0, x_0 + \delta), \abs*{x - x_0} < \delta' \implies \abs*{\frac{f(x) - f(x_0)}{x - x_0} - f'(x_0)} \leq \varepsilon
    \]
    and
    \[
        \forall\ x \in (a, b) \cap (x_0 - \delta, x_0), \abs*{x - x_0} < \delta' \implies \abs*{\frac{f(x) - f(x_0)}{x - x_0} - f'(x_0)} \leq \varepsilon.
    \]
    Thus by Definition \ref{9.3.6} we must have
    \[
        \lim_{x \to x_0 ; x \in (a, b) \cap (x_0, x_0 + \delta)} \frac{f(x) - f(x_0)}{x - x_0} = \lim_{x \to x_0 ; x \in (a, b) \cap (x_0 - \delta, x_0)} \frac{f(x) - f(x_0)}{x - x_0} = f'(x_0).
    \]
    Since
    \begin{align*}
                 & \forall\ x \in (a, b) \cap (x_0, x_0 + \delta)                                                                                       \\
        \implies & f(x) \leq f(x_0)                                                                                                                     \\
        \implies & f(x) - f(x_0) \leq 0                                                                                                                 \\
        \implies & \frac{f(x) - f(x_0)}{x - x_0} \leq 0                                                                                                 \\
        \implies & \lim_{x \to x_0 ; x \in (a, b) \cap (x_0, x_0 + \delta)} \frac{f(x) - f(x_0)}{x - x_0} \leq 0 & \text{(by Proposition \ref{9.3.14})} \\
        \implies & f'(x_0) \leq 0
    \end{align*}
    and
    \begin{align*}
                 & \forall\ x \in (a, b) \cap (x_0 - \delta, x_0)                                                                                        \\
        \implies & f(x) \leq f(x_0)                                                                                                                      \\
        \implies & f(x) - f(x_0) \leq 0                                                                                                                  \\
        \implies & \frac{f(x) - f(x_0)}{x - x_0} \geq 0                                                                                                  \\
        \implies & \lim_{x \to x_0 ; x \in (a, b) \cap (x_0 - \delta, x_0)} \frac{f(x) - f(x_0)}{x - x_0} \geq 0, & \text{(by Proposition \ref{9.3.14})} \\
        \implies & f'(x_0) \geq 0,
    \end{align*}
    we must have \(f'(x_0) = 0\).
    Similar arguments work for the case \(f\) attains local minimum at \(x_0\).
\end{proof}

\begin{note}
    \(f\) must be differentiable for Proposition \ref{10.2.6} to work.
    Also, Proposition \ref{10.2.6} does not work if the open interval \((a, b)\) is replaced by a closed interval \([a, b]\).
    For instance, the function \(f : [1, 2] \to \mathbf{R}\) defined by \(f(x) \coloneqq x\) has a local maximum at \(x_0 = 2\) and a local minimum \(x_0 = 1\) (in fact, these local extrema are global extrema), but at both points the derivative is \(f'(x_0) = 1\), not \(f'(x_0) = 0\).
    Thus the endpoints of an interval can be local maxima or minima even if the derivative is not zero there.
    Finally, the converse of this proposition is false.
\end{note}

\begin{theorem}[Rolle's theorem]\label{10.2.7}
    Let \(a < b\) be real numbers, and let \(g : [a, b] \to \mathbf{R}\) be a continuous function which is differentiable on \((a, b)\).
    Suppose also that \(g(a) = g(b)\).
    Then there exists an \(x \in (a, b)\) such that \(g'(x) = 0\).
\end{theorem}

\begin{proof}
    Since \(g\) is continuous on \([a, b]\), by Proposition \ref{9.6.7} \(g\) attains its maximum at some point \(x_{\max} \in [a, b]\), and also attains its minimum at some point \(x_{\min} \in [a, b]\).
    If \((x_{\min} \in \{a, b\}) \land (x_{\max} \in \{a, b\})\) is true, then by Definition \ref{9.6.5} we have \(g(x) = g(a) = g(b)\) for every \(x \in [a, b]\), and by Theorem \ref{10.1.13}(a) we know that \(g'(x) = 0\).
    So suppose that at least one of \(x_{\min}, x_{\max} \notin \{a, b\}\), i.e., \(\big(x_{\min} \in (a, b)\big) \lor \big(x_{\max} \in (a, b)\big)\) is true.
    If \(x_{\min} \in (a, b)\), then by Proposition \ref{10.2.6} we know that \(f'(x_{\min}) = 0\).
    Similarly, if \(x_{\max} \in (a, b)\), then by Proposition \ref{10.2.6} we know that \(f'(x_{\max}) = 0\).
    Thus there exists an \(x \in (a, b)\) such that \(g'(x) = 0\).
\end{proof}

\begin{remark}\label{10.2.8}
    We only assume \(f\) is differentiable on the open interval \((a, b)\), though of course Theorem \ref{10.2.7} also holds if we assume \(f\) is differentiable on the closed interval \([a, b]\), since this is larger than \((a, b)\).
\end{remark}

\begin{corollary}[Mean value theorem]\label{10.2.9}
    Let \(a < b\) be real numbers, and let \(f : [a, b] \to \mathbf{R}\) be a function which is continuous on \([a, b]\) and differentiable on \((a, b)\).
    Then there exists an \(x \in (a, b)\) such that \(f'(x) = \frac{f(b) - f(a)}{b - a}\).
\end{corollary}

\begin{proof}
    Let \(g : [a, b] \to \mathbf{R}\) be a function where \(g(x) = f(x) - \frac{f(a) - f(b)}{a - b} x\).
    Since \(a < b\), we know that \(g\) is well-defined.
    Since \(f\) is differentiable on \((a, b)\), we know that
    \begin{align*}
                 & x \text{ is differentiable on } (a, b)                                  & \text{(by Theorem \ref{10.1.13}(b))} \\
        \implies & \frac{f(a) - f(b)}{a - b} x \text{ is differentiable on } (a, b)        & \text{(by Theorem \ref{10.1.13}(e))} \\
        \implies & f(x) - \frac{f(a) - f(b)}{a - b} x \text{ is differentiable on } (a, b) & \text{(by Theorem \ref{10.1.13}(f))} \\
        \implies & g(x) \text{ is differentiable on } (a, b)                                                                      \\
        \implies & g'(x) = f'(x) - \frac{f(a) - f(b)}{a - b}.
    \end{align*}
    Since
    \[
        g(a) = f(a) - \frac{f(a) - f(b)}{a - b} a = \frac{af(a) - bf(a) - af(a) + af(b)}{a - b} = \frac{af(b) - bf(a)}{a - b}
    \]
    and
    \[
        g(b) = f(b) - \frac{f(a) - f(b)}{a - b} b = \frac{af(b) - bf(b) - bf(a) + bf(b)}{a - b} = \frac{af(b) - bf(a)}{a - b},
    \]
    we have \(g(a) = g(b)\) and by Theorem \ref{10.2.7} \(\exists\ x_0 \in (a, b)\) such that \(g'(x_0) = 0\).
    Thus
    \begin{align*}
                 & g'(x_0) = 0                             \\
        \implies & f'(x_0) - \frac{f(a) - f(b)}{a - b} = 0 \\
        \implies & f'(x_0) = \frac{f(a) - f(b)}{a - b}.
    \end{align*}
\end{proof}

\exercisesection

\begin{exercise}\label{ex 10.2.1}
    Prove Proposition \ref{10.2.6}.
\end{exercise}

\begin{proof}
    See Proposition \ref{10.2.6}.
\end{proof}

\begin{exercise}\label{ex 10.2.2}
    Give an example of a function \(f : (-1, 1) \to \mathbf{R}\) which is continuous and attains a global maximum at \(0\), but which is not differentiable at \(0\).
    Explain why this does not contradict Proposition \ref{10.2.6}.
\end{exercise}

\begin{proof}
    Let \(f(x) = -\abs*{x}\).
    Then \(f\) is continuous and attains a global maximum at \(0\), but which is not differentiable at \(0\).
    The fact that \(f\) is not differentiable at \(0\) does not contradict to Proposition \ref{10.2.6}.
\end{proof}

\begin{exercise}\label{ex 10.2.3}
    Give an example of a function \(f : (-1, 1) \to \mathbf{R}\) which is differentiable, and whose derivative equals \(0\) at \(0\), but such that \(0\) is neither a local minimum nor a local maximum.
    Explain why this does not contradict Proposition \ref{10.2.6}.
\end{exercise}

\begin{proof}
    Let \(f(x) = x^3\).
    Then by Exercise \ref{ex 10.1.5} we know that \(f'(x) = 3x^2\).
    Then we have \(f(0) = 0\) and \(f'(0) = 0\).
    But \(f(x) < f(0)\) for every \(x \in (-1, 0)\) and \(f(x) > f(0)\) for every \(x \in (0, 1)\).
    Thus \(0\) is neither a local minimum nor a local maximum.
    This does not contradict to Proposition \ref{10.2.6} since \(0\) is not given to be a local minimum or local maximum.
\end{proof}

\begin{exercise}\label{ex 10.2.4}
    Prove Theorem \ref{10.2.7}.
\end{exercise}

\begin{proof}
    See Theorem \ref{10.2.7}.
\end{proof}

\begin{exercise}\label{ex 10.2.5}
    Use Theorem \ref{10.2.7} to prove Corollary \ref{10.2.9}.
\end{exercise}

\begin{proof}
    See Corollary \ref{10.2.9}.
\end{proof}

\begin{exercise}\label{ex 10.2.6}
    Let \(M > 0\), and let \(f : [a, b] \to \mathbf{R}\) be a function which is continuous on \([a, b]\) and differentiable on \((a, b)\), and such that \(\abs*{f'(x)} \leq M\) for all \(x \in (a, b)\) (i.e., the derivative of \(f\) is bounded).
    Show that for any \(x, y \in [a, b]\) we have the inequality \(\abs*{f(x) - f(y)} \leq M \abs*{x - y}\).
    Functions which obey the bound \(\abs*{f(x) - f(y)} \leq M \abs*{x - y}\) are known as \emph{Lipschitz continuous functions} with \emph{Lipschitz constant} \(M\);
    thus this exercise shows that functions with bounded derivative are Lipschitz continuous.
\end{exercise}

\begin{proof}
    Let \(x, y \in [a, b]\).
    If \(x = y\), then we have \(0 = \abs*{f(x) - f(y)} \leq M \abs*{x - y} = 0\).
    So suppose that \(x \neq y\).
    We have either \(x < y\) or \(x > y\).
    Without the loss of generality suppose that \(x < y\).
    Then we have \([x, y] \subseteq [a, b]\) and \((x, y) \subseteq (a, b)\).
    By Exercise \ref{ex 9.4.6} we know that \(f|_{[x, y]}\) is continuous on \([x, y]\).
    By Exercise \ref{ex 10.1.1} we know that \(f|_{[x, y]}\) is differentiable on \((x, y)\).
    By mean value theorem (Corollary \ref{10.2.9}) we know that \(\exists\ c \in (x, y)\) such that
    \[
        f'(c) = \frac{f(y) - f(x)}{y - x}.
    \]
    Since \(c \in (x, y)\), we have \(c \in (a, b)\).
    By hypothesis we have
    \begin{align*}
                 & \abs*{f'(c)} = \abs*{\frac{f(y) - f(x)}{y - x}} \leq M \\
        \implies & \abs*{f(y) - f(x)} \leq M \abs*{y - x}                 \\
        \implies & \abs*{f(x) - f(y)} \leq M \abs*{x - y}.
    \end{align*}
    Thus we conclude that \(\forall\ x, y \in [a, b]\), we have \(\abs*{f(x) - f(y)} \leq M \abs*{x - y}\).
\end{proof}

\begin{exercise}\label{ex 10.2.7}
    Let \(f : \mathbf{R} \to \mathbf{R}\) be a differentiable function such that \(f'\) is bounded.
    Show that \(f\) is uniformly continuous.
\end{exercise}

\begin{proof}
    Since \(f'\) is bounded, by Definition \ref{9.6.1} we know that \(\exists\ M \in \mathbf{R}^+\) such that \(\abs*{f'(x)} \leq M\) for every \(x \in \mathbf{R}\).
    By Exercise \ref{ex 10.2.6} we know that \(\abs*{f(x) - f(y)} \leq M \abs*{x - y}\) for every \(x, y \in \mathbf{R}\).
    Then we have
    \begin{align*}
                 & \forall\ \varepsilon \in \mathbf{R}^+, \exists\ \delta = \varepsilon / M : \forall\ x, y \in \mathbf{R}, \abs*{x - y} \leq \delta \\
        \implies & \abs*{f(x) - f(y)} \leq M \abs*{x - y} \leq M \delta = M \frac{\varepsilon}{M} = \varepsilon
    \end{align*}
    and by Definition \ref{9.9.2} \(f\) is uniformly continuous.
\end{proof}