\section{Convergence and limit laws}

\begin{definition}[Distance between two real numbers]\label{6.1.1}
Given two real numbers \(x\) and \(y\), we define their distance \(d(x, y)\) to be \(d(x, y) \coloneqq \abs*{x - y}\).
\end{definition}

\begin{note}
Clearly Definition \ref{6.1.1} is consistent with Definition \ref{4.3.2}.
Further, Proposition \ref{4.3.3} works just as well for real numbers as it does for rationals, because the real numbers obey all the rules of algebra that the rationals do.
\end{note}

\begin{definition}[\(\varepsilon\)-close real numbers]\label{6.1.2}
Let \(\varepsilon > 0\) be a real number.
We say that two real numbers \(x, y\) are \emph{\(\varepsilon\)-close} iff we have \(d(y, x) \leq \varepsilon\).
\end{definition}

\begin{note}
Again, it is clear that Definition \ref{6.1.2} is consistent with Definition \ref{4.3.4}.
\end{note}

\begin{note}
Now let \((a_n)_{n = m}^\infty\) be a sequence of real numbers;
i.e., we assign a real number \(a_n\) for every integer \(n \geq m\).
The starting index \(m\) is some integer;
usually this will be \(1\), but in some cases we will start from some index other than \(1\).
(The choice of label used to index this sequence is unimportant; we could use for instance \((a_k)_{k = m}^{\infty}\) and this would represent exactly the same sequence as \((a_n)_{n = m}^{\infty}\).
We can define the notion of a Cauchy sequence in the same manner as before.
\end{note}

\begin{definition}[Cauchy sequences of reals]\label{6.1.3}
Let \(\varepsilon > 0\) be a real number.
A sequence \((a_n)_{n = N}^\infty\) of real numbers starting at some integer index \(N\) is said to be \emph{\(\varepsilon\)-steady} iff \(a_j\) and \(a_k\) are \(\varepsilon\)-close for every \(j, k \geq N\).
A sequence \((a_n)_{n = m}^\infty\) starting at some integer index \(m\) is said to be \emph{eventually \(\varepsilon\)-steady} iff there exists an \(N \geq m\) such that \((a_n)_{n = N}^\infty\) is \(\varepsilon\)-steady.
We say that \((a_n)_{n = m}^\infty\) is a \emph{Cauchy sequence} iff it is eventually \(\varepsilon\)-steady for every \(\varepsilon > 0\).
\end{definition}

\begin{note}
To put it another way, a sequence \((a_n)_{n = m}^\infty\) of real numbers is a Cauchy sequence if, for every real \(\varepsilon > 0\), there exists an \(N \geq m\) such that \(\abs*{a_n - a_n'} \leq \varepsilon\) for all \(n, n' \geq N\).
These definitions are consistent with the corresponding definitions for rational numbers (Definitions \ref{5.1.3}, \ref{5.1.6}, \ref{5.1.8}), although verifying consistency for Cauchy sequences takes a little bit of care.
\end{note}

\begin{proposition}\label{6.1.4}
Let \((a_n)_{n = m}^\infty\) be a sequence of rational numbers starting at some integer index \(m\).
Then \((a_n)_{n = m}^\infty\) is a Cauchy sequence in the sense of Definition \ref{5.1.8} if and only if it is a Cauchy sequence in the sense of Definition \ref{6.1.3}.
\end{proposition}

\begin{proof}
Suppose first that \((a_n)_{n = m}^\infty\) is a Cauchy sequence in the sense of Definition \ref{6.1.3};
then it is eventually \(\varepsilon\)-steady for every real \(\varepsilon > 0\).
In particular, it is eventually \(\varepsilon\)-steady for every rational \(\varepsilon > 0\), which makes it a Cauchy sequence in the sense of Definition \ref{5.1.8}.

Now suppose that \((a_n)_{n = m}^\infty\) is a Cauchy sequence in the sense of Definition \ref{5.1.8};
then it is eventually \(\varepsilon\)-steady for every rational \(\varepsilon > 0\).
If \(\varepsilon > 0\) is a real number, then there exists a rational \(\varepsilon' > 0\) which is smaller than \(\varepsilon\), by Proposition \ref{5.4.12}.
Since \(\varepsilon'\) is rational, we know that \((a_n)_{n = m}^\infty\) is eventually \(\varepsilon'\)-steady;
since \(\varepsilon' < \varepsilon\), this implies that \((a_n)_{n = m}^\infty\) is eventually \(\varepsilon\)-steady.
Since \(\varepsilon\) is an arbitrary positive real number, we thus see that \((a_n)_{n = m}^\infty\) is a Cauchy sequence in the sense of Definition \ref{6.1.3}.
\end{proof}

\begin{note}
Because of Proposition \ref{6.1.4}, we will no longer care about the distinction between Definition \ref{5.1.8} and Definition \ref{6.1.3}, and view the concept of a Cauchy sequence as a single unified concept.
\end{note}

\begin{definition}[Convergence of sequences]\label{6.1.5}
Let \(\varepsilon > 0\) be a real number, and let \(L\) be a real number.
A sequence \((a_n)_{n = N}^\infty\) of real numbers is said to be \emph{\(\varepsilon\)-close to \(L\)} iff \(a_n\) is \(\varepsilon\)-close to \(L\) for every \(n \geq N\), i.e., we have \(\abs*{a_n - L} \leq \varepsilon\) for every \(n \geq N\).
We say that a sequence \((a_n)_{n = m}^\infty\) is \emph{eventually \(\varepsilon\)-close to \(L\)} iff there exists an \(N \geq m\) such that \((a_n)_{n = N}^\infty\) is \(\varepsilon\)-close to \(L\).
We say that a sequence \((a_n)_{n = m}^\infty\) \emph{converges to \(L\)} iff it is eventually \(\varepsilon\)-close to \(L\) for every real \(\varepsilon > 0\).
\end{definition}

\setcounter{theorem}{6}
\begin{proposition}[Uniqueness of limits]\label{6.1.7}
Let \((a_n)_{n = m}^\infty\) be a real sequence starting at some integer index \(m\), and let \(L \neq L'\) be two distinct real numbers.
Then it is not possible for \((a_n)_{n = m}^\infty\) to converge to \(L\) while also converging to \(L'\).
\end{proposition}

\begin{proof}
Suppose for sake of contradiction that \((a_n)_{n = m}^\infty\) was converging to both \(L\) and \(L'\).
Let \(\varepsilon = \abs*{L - L'} / 3\);
note that \(\varepsilon\) is positive since \(L \neq L'\).
Since \((a_n)_{n = m}^\infty\) converges to \(L\), we know that \((a_n)_{n = m}^\infty\) is eventually \(\varepsilon\)-close to \(L\);
thus there is an \(N \geq m\) such that \(d(a_n, L) \leq \varepsilon\) for all \(n \geq N\).
Similarly, there is an \(M \geq m\) such that \(d(a_n, L') \leq \varepsilon\) for all \(n \geq M\).
In particular, if we set \(n \coloneqq \max(N, M)\), then we have \(d(a_n, L) \leq \varepsilon\) and \(d(a_n, L') \leq \varepsilon\), hence by the triangle inequality \(d(L, L') \leq 2\varepsilon = 2\abs*{L - L'} / 3\).
But then we have \(\abs*{L - L'} \leq 2\abs*{L - L'} / 3\), which contradicts the fact that \(\abs*{L - L'} > 0\).
Thus it is not possible to converge to both \(L\) and \(L'\).
\end{proof}

\begin{definition}[Limits of sequences]\label{6.1.8}
If a sequence \((a_n)_{n = m}^\infty\) converges to some real number \(L\), we say that \((a_n)_{n = m}^\infty\) is \emph{convergent} and that its \emph{limit} is \(L\);
we write
\[
    L = \lim_{n \to \infty} a_n
\]
to denote this fact.
If a sequence \((a_n)_{n = m}^\infty\) is not converging to any real number \(L\), we say that the sequence \((a_n)_{n = m}^\infty\) is \emph{divergent} and we leave \(\lim_{n \to \infty} a_n\) undefined.
\end{definition}

\begin{note}
Proposition \ref{6.1.7} ensures that a sequence can have at most one limit.
Thus, if the limit exists, it is a single real number, otherwise it is undefined.
\end{note}

\begin{remark}\label{6.1.9}
The notation \(\lim_{n \to \infty} a_n\) does not give any indication about the starting index \(m\) of the sequence, but the starting index is irrelevant.
Thus in the rest of this discussion we shall not be too careful as to where these sequences start, as we shall be mostly focused on their limits.
\end{remark}

\begin{note}
We sometimes use the phrase ``\(a_n \to x\) as \(n \to \infty\)'' as an alternate way of writing the statement ``\((a_n)_{n = m}^\infty\) converges to \(x\)''.
Bear in mind, though, that the individual statements \(a_n \to x\) and \(n \to \infty\) do not have any rigorous meaning;
this phrase is just a convention, though of course a very suggestive one.
\end{note}

\begin{remark}\label{6.1.10}
The exact choice of letter used to denote the index (in this case \(n\)) is irrelevant:
the phrase \(\lim_{n \to \infty} a_n\) has exactly the same meaning as \(\lim_{k \to \infty} a_k\), for instance.
Sometimes it will be convenient to change the label of the index to avoid conflicts of notation;
for instance, we might want to change \(n\) to \(k\) because \(n\) is simultaneously being used for some other purpose, and we want to reduce confusion.
\end{remark}

\exercisesection

\begin{exercise}\label{ex 6.1.1}
Let \((a_n)_{n = m}^\infty\) be a sequence of real numbers, such that \(a_{n + 1} > a_n\) for each natural number \(n\).
Prove that whenever \(n\) and \(m\) are natural numbers such that \(m > n\), then we have \(a_m > a_n\).
(We refer to these sequences as \emph{increasing} sequences.)
\end{exercise}

\begin{proof}
Let \(E = \{z \in \mathds{N} : n \leq z \leq m\}\).
Then \(E\) is a finite set since \(m - n \in \mathds{N}\) and is non-empty set since \(n, m \in E\).
Let \((a_z)_{z = n}^m\) be a sequence by mapping \(z \in E\) to \(a_z\).
So \((a_z)_{z = n}^m\) is a finite sequence, and the elements in sequence \((a_z)_{z = n}^m\) are \(\{a_n, a_{n + 1}, \dots, a_{m - 1}, a_m\}\).
By the given conditions we have \(a_{z + 1} > a_z\) for each natural number \(z\).
Thus we have \(a_n < a_{n + 1} < \dots < a_{m - 1} < a_m\), and by Proposition \ref{5.4.7} we have \(a_n < a_m\).
\end{proof}

\begin{exercise}\label{ex 6.1.2}
Let \((a_n)_{n = m}^\infty\) be a sequence of real numbers, and let \(L\) be a real number.
Show that \((a_n)_{n = m}^\infty\) converges to \(L\) if and only if, given any real \(\varepsilon > 0\), one can find an \(N \geq m\) such that \(\abs*{a_n - L} \leq \varepsilon\) for all \(n \geq N\).
\end{exercise}

\begin{proof}
\begin{align*}
& (a_n)_{n = m}^\infty \text{ converges to } L \\
\iff & (\forall\ (\varepsilon \in \mathds{R}) \land (\varepsilon > 0)), (a_n)_{n = m}^\infty \text{ is eventually } \varepsilon\text{-close to } L & \text{(by Definition \ref{6.1.5})} \\
\iff & (\forall\ (\varepsilon \in \mathds{R}) \land (\varepsilon > 0)), (\exists\ (N \in \mathds{N}) \land (N \geq m)) : \\
& (a_n)_{n = N}^\infty \text{ is } \varepsilon\text{-close to } L & \text{(by Definition \ref{6.1.5})} \\
\iff & (\forall\ (\varepsilon \in \mathds{R}) \land (\varepsilon > 0)), (\exists\ (N \in \mathds{N}) \land (N \geq m)) : \\
& \abs*{a_n - L} \leq \varepsilon \ \forall\ n \geq N. & \text{(by Definition \ref{6.1.5})}
\end{align*}
\end{proof}

\begin{exercise}\label{ex 6.1.3}
Let \((a_n)_{n = m}^\infty\) be a sequence of real numbers, let \(c\) be a real number, and let \(m' \geq m\) be an integer.
Show that \((a_n)_{n = m}^\infty\) converges to \(c\) if and only if \((a_n)_{n = m'}^\infty\) converges to \(c\).
\end{exercise}

\begin{proof}
We first show that if \((a_n)_{n = m}^\infty\) converges to \(c\), then \((a_n)_{n = m'}^\infty\) converges to \(c\).
\begin{align*}
& (a_n)_{n = m}^\infty \text{ converges to } c \\
\implies & (\forall\ (\varepsilon \in \mathds{R}) \land (\varepsilon > 0)), (a_n)_{n = m}^\infty \text{ is eventually } \varepsilon\text{-close to } c & \text{(by Definition \ref{6.1.5})} \\
\implies & (\forall\ (\varepsilon \in \mathds{R}) \land (\varepsilon > 0)), (\exists\ (N \in \mathds{N}) \land (N \geq m)) : \\
& (a_n)_{n = N}^\infty \text{ is } \varepsilon\text{-close to } c. & \text{(by Definition \ref{6.1.5})}
\end{align*}
Now we can divide into two cases:
\begin{enumerate}
    \item \(N \geq m'\).
    This means \(\forall\ \varepsilon \in \mathds{R}\) and \(\varepsilon > 0\), \(\exists\ N \in \mathds{N}\) and \(N \geq m'\) such that \((a_n)_{n = N}^\infty\) is \(\varepsilon\)-close to \(c\).
    Thus \((a_n)_{n = m'}^\infty\) converges to \(c\).
    \item \(N < m'\).
    Then we can let \(N = m'\), so \(\forall\ \varepsilon \in \mathds{R}\) and \(\varepsilon > 0\), \(\exists\ N \in \mathds{N}\) and \(N \geq m'\) such that \((a_n)_{n = N}^\infty\) is \(\varepsilon\)-close to \(c\).
    Thus \((a_n)_{n = m'}^\infty\) converges to \(c\).
\end{enumerate}
In both cases we get \((a_n)_{n = m'}^\infty\) converges to \(c\).
Thus if \((a_n)_{n = m}^\infty\) converges to \(c\), then \((a_n)_{n = m'}^\infty\) converges to \(c\).

Now we shows that if \((a_n)_{n = m'}^\infty\) converges to \(c\), then \((a_n)_{n = m}^\infty\) converges to \(c\).
\begin{align*}
& (a_n)_{n = m'}^\infty \text{ converges to } c \\
\implies & (\forall\ (\varepsilon \in \mathds{R}) \land (\varepsilon > 0)), (a_n)_{n = m}^\infty \text{ is eventually } \varepsilon\text{-close to } c & \text{(by Definition \ref{6.1.5})} \\
\implies & (\forall\ (\varepsilon \in \mathds{R}) \land (\varepsilon > 0)), (\exists\ (N \in \mathds{N}) \land (N \geq m')) : \\
& (a_n)_{n = N}^\infty \text{ is } \varepsilon\text{-close to } c & \text{(by Definition \ref{6.1.5})} \\
\implies & (\forall\ (\varepsilon \in \mathds{R}) \land (\varepsilon > 0)), (\exists\ (N \in \mathds{N}) \land (N \geq m)) : \\
& (a_n)_{n = N}^\infty \text{ is } \varepsilon\text{-close to } c & \text{(by Definition \ref{6.1.5})} \\
\implies & (a_n)_{n = m}^\infty \text{ converges to } c.
\end{align*}
Thus if \((a_n)_{n = m'}^\infty\) converges to \(c\), then \((a_n)_{n = m}^\infty\) converges to \(c\).
We conclude that \((a_n)_{n = m}^\infty\) converges to \(c\) if and only if \((a_n)_{n = m'}^\infty\) converges to \(c\).
\end{proof}

\begin{exercise}\label{ex 6.1.4}
Let \((a_n)_{n = m}^\infty\) be a sequence of real numbers, let \(c\) be a real number, and let \(k \geq 0\) be a non-negative integer.
Show that \((a_n)_{n = m}^\infty\) converges to \(c\) if and only if \((a_{n + k})_{n = m}^\infty\) converges to \(c\).
\end{exercise}

\begin{proof}
Since \((a_{n + k})_{n = m}^\infty = (a_n)_{n = m + k}^\infty\) and \(m + k \geq m\), by Exercise \ref{ex 6.1.3} we have \((a_n)_{n = m}^\infty\) converges to \(c\) if and only if \((a_n)_{n = m + k}^\infty\) converges to \(c\).
Thus \((a_n)_{n = m}^\infty\) converges to \(c\) if and only if \((a_{n + k})_{n = m}^\infty\) converges to \(c\).
\end{proof}