\section{The Extended real number system}\label{sec 6.2}

\begin{definition}[Extended real number system]\label{6.2.1}
The \emph{extended real number system \(\mathds{R}^*\)} is the real line \(\mathds{R}\) with two additional elements attached, called \(+\infty\) and \(-\infty\).
These elements are distinct from each other and also distinct from every real number.
An extended real number \(x\) is called \emph{finite} iff it is a real number, and \emph{infinite} iff it is equal to \(+\infty\) or \(-\infty\).
(This definition is not directly related to the notion of finite and infinite sets in Section \ref{sec 3.6}, though it is of course similar in spirit.)
\end{definition}

\begin{definition}[Negation of extended reals]\label{6.2.2}
The operation of negation \(x \to -x\) on \(\mathds{R}\), we now extend to \(\mathds{R}^*\) by defining \(-(+\infty) \coloneqq -\infty\) and \(-(-\infty) \coloneqq +\infty\).
\end{definition}

\begin{note}
Thus every extended real number \(x\) has a negation, and \(-(-x)\) is always equal to \(x\).
\end{note}

\begin{definition}[Ordering of extended reals]\label{6.2.3}
Let \(x\) and \(y\) be extended real numbers.
We say that \(x \leq y\), i.e., \(x\) is less than or equal to \(y\), iff one of the following three statements is true:
\begin{enumerate}
    \item \(x\) and \(y\) are real numbers, and \(x \leq y\) as real numbers.
    \item \(y = +\infty\).
    \item \(x = -\infty\).
\end{enumerate}
We say that \(x < y\) if we have \(x \leq y\) and \(x \neq y\).
We sometimes write \(x < y\) as \(y > x\), and \(x \leq y\) as \(y \geq x\).
\end{definition}

\setcounter{theorem}{4}
\begin{proposition}\label{6.2.5}
Let \(x, y, z\) be extended real numbers.
Then the following statements are true:
\begin{enumerate}
    \item (Reflexivity)
    We have \(x \leq x\).
    \item (Trichotomy)
    Exactly one of the statements \(x < y\), \(x = y\), or \(x > y\) is true.
    \item (Transitivity)
    If \(x \leq y\) and \(y \leq z\), then \(x \leq z\).
    \item (Negation reverses order) If \(x \leq y\), then \(-y \leq -x\).
\end{enumerate}
\end{proposition}

\begin{proof}{(a)}
By Proposition \ref{5.4.7}, we already have \(x \leq x\) when \(x \in \mathds{R}\).
So we only need to consider the cases \(x = +\infty\) or \(x = -\infty\).
By Definition \ref{6.2.3}, we have \(x \leq +\infty \ \forall\ x \in \mathds{R}^*\).
So we have \(+\infty \leq +\infty\).
Again by Definition \ref{6.2.3}, we have \(-\infty \leq x \ \forall\ x \in \mathds{R}^*\).
So we have \(-\infty \leq -\infty\).
Thus we conclude that \(x \leq x \ \forall\ x \in \mathds{R}^*\).
\end{proof}

\begin{proof}{(b)}
By Proposition \ref{5.4.7}, we already have exactly one of the statements \(x < y\), \(x = y\), or \(x > y\) is true when \(x, y \in \mathds{R}\).
So we only need to consider the cases \(x = +\infty\), \(x = -\infty\), \(y = +\infty\), or \(y = -\infty\).
\begin{enumerate}[label=(\Roman*)]
    \item If \(x = +\infty\), then by Definition \ref{6.2.3} we have \(x \geq y \ \forall\ y \in \mathds{R}^*\).
    \begin{enumerate}[label=(\roman*)]
        \item If \(y = +\infty\), then we have \(x = y\).
        \item If \(y \in \mathds{R}\), then by Definition \ref{6.2.1} \(x \neq y\).
        Thus by Definition \ref{6.2.3} we have \(x > y\).
        \item If \(y = -\infty\), then by Definition \ref{6.2.1} \(x \neq y\).
        Thus by Definition \ref{6.2.3} we have \(x > y\).
    \end{enumerate}
    \item If \(x = -\infty\), then by Definition \ref{6.2.3} we have \(x \leq y \ \forall\ y \in \mathds{R}^*\).
    \begin{enumerate}[label=(\roman*)]
        \item If \(y = +\infty\), then by Definition \ref{6.2.1} \(x \neq y\).
        Thus by Definition \ref{6.2.3} we have \(x < y\).
        \item If \(y \in \mathds{R}\), then by Definition \ref{6.2.1} \(x \neq y\).
        Thus by Definition \ref{6.2.3} we have \(x < y\).
        \item If \(y = -\infty\), then we have \(x = y\).
    \end{enumerate}
    \item If \(y = +\infty\), then by Definition \ref{6.2.3} we have \(x \leq y \ \forall\ x \in \mathds{R}^*\).
    \begin{enumerate}[label=(\roman*)]
        \item If \(x = +\infty\), then we have \(x = y\).
        \item If \(x \in \mathds{R}\), then by Definition \ref{6.2.1} \(x \neq y\).
        Thus by Definition \ref{6.2.3} we have \(x < y\).
        \item If \(x = -\infty\), then by Definition \ref{6.2.1} \(x \neq y\).
        Thus by Definition \ref{6.2.3} we have \(x < y\).
    \end{enumerate}
    \item If \(y = -\infty\), then by Definition \ref{6.2.3} we have \(x \geq y \ \forall\ x \in \mathds{R}^*\).
    \begin{enumerate}[label=(\roman*)]
        \item If \(x = +\infty\), then by Definition \ref{6.2.1} \(x \neq y\).
        Thus by Definition \ref{6.2.3} we have \(x > y\).
        \item If \(x \in \mathds{R}\), then by Definition \ref{6.2.1} \(x \neq y\).
        Thus by Definition \ref{6.2.3} we have \(x > y\).
        \item If \(x = -\infty\), then we have \(x = y\).
    \end{enumerate}
\end{enumerate}
From all cases above we show that exactly one of the statements \(x < y\), \(x = y\), or \(x > y\) is true.
Thus we finish the proof.
\end{proof}

\begin{proof}{(c)}
By Proposition \ref{5.4.7}, we already have \((x \leq y) \land (y \leq z) \implies x \leq z\) when \(x, y, z \in \mathds{R}\).
So we only need to consider the cases \(x = +\infty\), \(x = -\infty\), \(y = +\infty\), \(y = -\infty\), \(z = +\infty\), or \(z = -\infty\).
\begin{enumerate}[label=(\Roman*)]
    \item If \(x = +\infty\), then by Definition \ref{6.2.3} \((x = +\infty) \land (x \leq y) \implies y = +\infty\).
    Similarly \((y = +\infty) \land (y \leq z) \implies z = +\infty\).
    Thus we have \(x = +\infty = z\), and by Proposition \ref{6.2.5}(a) we have \(x \leq z\).
    \item If \(x = -\infty\), then by Definition \ref{6.2.3} \(x \leq z \ \forall\ z \in \mathds{R}^*\).
    \item If \(y = +\infty\), then by Definition \ref{6.2.3} \((y = +\infty) \land (y \leq z) \implies z = +\infty\).
    Again by Definition \ref{6.2.3}, we have \(x \leq +\infty = z \ \forall\ x \in \mathds{R}^*\).
    \item If \(y = -\infty\), then by Definition \ref{6.2.3} \((y = -\infty) \land (x \leq y) \implies x = -\infty\).
    Again by Definition \ref{6.2.3}, we have \(x = -\infty \leq z \ \forall\ z \in \mathds{R}^*\).
    \item If \(z = +\infty\), then by Definition \ref{6.2.3}, we have \(x \leq +\infty = z \ \forall\ x \in \mathds{R}^*\).
    \item If \(z = -\infty\), then by Definition \ref{6.2.3} \((z = -\infty) \land (y \leq z) \implies y = -\infty\).
    Similarly \((y = -\infty) \land (x \leq y) \implies x = -\infty\).
    Thus we have \(x = -\infty = z\), and by Proposition \ref{6.2.5}(a) we have \(x \leq z\).
\end{enumerate}
From all cases above we show that \((x \leq y) \land (y \leq z) \implies x \leq z\).
Thus we finish the proof.
\end{proof}

\begin{proof}{(d)}
By Proposition \ref{5.4.7}, we already have \(x \leq y \implies -y \leq -x\) when \(x, y \in \mathds{R}\).
So we only need to consider the cases \(x = +\infty\), \(x = -\infty\), \(y = +\infty\), or \(y = -\infty\).
\begin{enumerate}[label=(\Roman*)]
    \item If \(x = +\infty\), then by Definition \ref{6.2.3} \((x = +\infty) \land (x \leq y) \implies y = +\infty\).
    And by Definition \ref{6.2.2} we have \(-x = -\infty = -y\).
    Thus by Proposition \ref{6.2.5}(a) we have \(-y \leq -x\).
    \item If \(x = -\infty\), then by Definition \ref{6.2.2} \(-x = +\infty\).
    And by Definition \ref{6.2.3} we have \(-y \leq -x \ \forall\ -y \in \mathds{R}^*\).
    \item If \(y = +\infty\), then by Definition \ref{6.2.2} \(-y = -\infty\).
    And by Definition \ref{6.2.3} we have \(-y \leq -x \ \forall\ -x \in \mathds{R}^*\).
    \item If \(y = -\infty\), then by Definition \ref{6.2.3} \((y = -\infty) \land (x \leq y) \implies x = -\infty\).
    And by Definition \ref{6.2.2} we have \(-x = +\infty = -y\).
    Thus by Proposition \ref{6.2.5}(a) we have \(-y \leq -x\).
\end{enumerate}
From all cases above we show that \(x \leq y \implies -y \leq -x\).
Thus we finish the proof.
\end{proof}

\exercisesection

\begin{exercise}\label{ex 6.2.1}
Prove Proposition \ref{6.2.5}.
\end{exercise}

\begin{proof}
See Proposition \ref{6.2.5}.
\end{proof}