\section{Subsequences}\label{sec 6.6}

\begin{definition}[Subsequences]\label{6.6.1}
Let \((a_n)_{n = 0}^\infty\) and \((b_n)_{n = 0}^\infty\) be sequences of real numbers.
We say that \((b_n)_{n = 0}^\infty\) is a \emph{subsequence} of \((a_n)_{n = 0}^\infty\) iff there exists a function \(f : \mathbf{N} \to \mathbf{N}\) which is strictly increasing (i.e., \(f(n + 1) > f(n)\) for all \(n \in \mathbf{N}\)) such that
\[
    b_n = a_{f(n)} \text{ for all } n \in \mathbf{N}.
\]
\end{definition}

\setcounter{theorem}{3}
\begin{lemma}\label{6.6.4}
Let \((a_n)_{n = 0}^\infty\) and \((b_n)_{n = 0}^\infty\) be sequences of real numbers.
Then \((a_n)_{n = 0}^\infty\) is a subsequence of \((a_n)_{n = 0}^\infty\).
Furthermore, if \((b_n)_{n = 0}^\infty\) is a subsequence of \((a_n)_{n = 0}^\infty\), and \((c_n)_{n = 0}^\infty\) is a subsequence of \((b_n)_{n = 0}^\infty\), then \((c_n)_{n = 0}^\infty\) is a subsequence of \((a_n)_{n = 0}^\infty\).
\end{lemma}

\begin{proof}
We first show that \((a_n)_{n = 0}^\infty\) is a subsequence of \((a_n)_{n = 0}^\infty\).
Let \(f : \mathbf{N} \to \mathbf{N}\) be a function where \(f(n) = n\).
Since \(f\) is strictly increasing, \((a_n)_{n = 0}^\infty\) is a subsequence of \((a_n)_{n = 0}^\infty\).

Now we show that if \((b_n)_{n = 0}^\infty\) is a subsequence of \((a_n)_{n = 0}^\infty\), and \((c_n)_{n = 0}^\infty\) is a subsequence of \((b_n)_{n = 0}^\infty\), then \((c_n)_{n = 0}^\infty\) is a subsequence of \((a_n)_{n = 0}^\infty\).
Since \((b_n)_{n = 0}^\infty\) is a subsequence of \((a_n)_{n = 0}^\infty\), \(\exists\ f : \mathbf{N} \to \mathbf{N}\) such that \(f\) is strictly increasing and \(b_n = a_{f(n)}\).
Since \((c_n)_{n = 0}^\infty\) is a subsequence of \((b_n)_{n = 0}^\infty\), \(\exists\ g : \mathbf{N} \to \mathbf{N}\) such that \(f\) is strictly increasing and \(c_n = b_{g(n)}\).
Let \(h = g \circ f\).
Since \(f\) is strictly increasing, \(n_1 < n_2 \implies f(n_1) < f(n_2)\).
Since \(g\) is strictly increasing, \(f(n_1) < f(n_2) \implies g(f(n_1)) < g(f(n_2))\).
Thus \(h\) is also strictly increasing, and \((c_n)_{n = 0}^\infty\) is a subsequence of \((a_n)_{n = 0}^\infty\) where \(c_n = a_{g(f(n))}\).
\end{proof}

\exercisesection

\begin{exercise}\label{6.6.1}
Prove Lemma \ref{6.6.4}.
\end{exercise}

\begin{proof}
See Lemma \ref{6.6.4}.
\end{proof}